\documentclass{report}
\usepackage{amsmath}
\usepackage{amssymb}
\usepackage[version=4]{mhchem}

\begin{document}
     $\hat{H} = \hslash [ D (\hat{S}_z^2 - \frac{2}{3} I_3) + E (\hat{S}_x^2 - \hat{S}_y^2) + \gamma_{nv} \vec{B} \cdot \hat{\vec{S}} ]$\\
     $\Delta E_{[m_s = +1]} = + g_e \mu_B \mid \vec{B} \cdot \hat{u} \mid$ \\
     $\Delta E_{[m_s = -1]} = - g_e \mu_B \mid\vec{B} \cdot \hat{u} \mid$ \\
     $\Delta E_{[m_s = 0]} = 0$ \\
     $\hat{H} = \hslash [ D (\hat{S}_z^2 - \frac{2}{3} I_3) + \gamma_{nv} B_z \hat{S}_z ]$\\
     $m_s = +1$ \\
     $m_s = -1$ \\
     $\Delta \nu_i = {\nu_i}_{[+1]} - {\nu_i}_{[-1]} $ \\
     $B_i = \Delta \nu_i / \gamma_{nv} $ \\
     \begin{equation}
      \begin{cases}
        \Delta \nu_i = {\nu_i}_{[+1]} - {\nu_i}_{[-1]} \\ \\
        B_i = \Delta \nu_i / \gamma_{nv} 
      \end{cases}  
     \end{equation}
      
    $[\hat{u}_1,\hat{u}_2,\hat{u}_3,\hat{u}_4];[-1,-1, \ 1, \ 1]$

     \begin{equation}
      \begin{cases}
        \vec{B} \cdot \hat{u}_{list}[i]_1 = B_1 \\
        \vec{B} \cdot \hat{u}_{list}[i]_2 = B_2 \\
        \vec{B} \cdot \hat{u}_{list}[i]_3 = B_3 \\
      \end{cases}  
     \end{equation}

     \begin{equation}
      \begin{cases}
        \vec{B} \cdot \hat{u}_1 = B_i \\
        \vec{B} \cdot \hat{u}_2 = B_i \\
        \vec{B} \cdot \hat{u}_3 = B_i \\
      \end{cases}  
     \end{equation}

    $\vec{B} \cdot \hat{u}_{list}[i]_4 = B_4$ \\
\end{document}
